\section{Advection}
\subsection{Differential equation}
\begin{equation}
	\bLaplacian C - \alpha \mathbf{V} \bcdot \bnabla C = 0	
\end{equation}

\subsection{1D example}
\begin{eqnarray}
  f'' - \alpha f' = 0 \\
  f(0) = 0 \\ f(1) = 1
\end{eqnarray}
Use $f(x) = e^{\gamma x}$ so $\gamma \in \{0, \alpha\}$ so:
\begin{eqnarray}
  f(x) &=& Ae^{\alpha x} + B \\
  0 &=& A + B \\
  1 &=& Ae^{\alpha} + B
\end{eqnarray}
The continuous solution is:
\begin{eqnarray}
  f(x) &=& \frac{e^{\alpha x} - 1}{e^{\alpha} - 1}
\end{eqnarray}

\subsection{Central difference}
We start by using the following scheme:
\begin{eqnarray}
  \frac{f_{k-1}-2f_k+f_{k+1}}{h^2}
  - \alpha \frac{f_{k+1}-f_{k-1}}{2h} &=& 0 \\
(f_{k-1}-2f_k+f_{k+1}) - \eps (f_{k+1}-f_{k-1}) &=& 0 \\
\eps = \frac{\alpha h}{2} \\
(1-\eps)f_{k-1}-2f_k+(1+\eps)f_{k+1} &=& 0
\end{eqnarray}
Write $f_k = \gamma^k$ to get:
\begin{eqnarray}
  (1-\eps)\gamma^{k-1} - 2\gamma^k + (1+\eps)\gamma^{k+1}&=& 0 \\
  (1-\eps)\gamma - 2\gamma + (1+\eps)\gamma^2&=& 0 \\
  \gamma = \frac{1 \pm \sqrt{1 - (1-\eps)(1+\eps)}}{1+\eps}
         = \frac{1 \pm |\eps|}{1+\eps} \in
           \left\{1, \frac{1- \eps}{1+\eps}\right\}
\end{eqnarray}
Take $f_0 = 0$ and $f_N = 1$ such that $h N = 1$, so:
\begin{eqnarray}
  f_k &=& \frac{1 - \left(\frac{1- \eps}{1+\eps}\right)^k}
  {1 - \left(\frac{1- \eps}{1+\eps}\right)^N}
\end{eqnarray}
Denote $x = \frac{k}{N}$ for $|\eps| < 1$:
\begin{eqnarray}
(1+\eps)^k = \left(1+\frac{\alpha h}{2}\right)^k =
\left(1+\frac{\alpha}{2N}\right)^k =
\left(1+\frac{\frac{\alpha k}{2N}}{k}\right)^k \approx
e^{\frac{\alpha k}{2N}} = e^{\frac{\alpha x}{2}}
\end{eqnarray}
So:
\begin{eqnarray}
  \left(\frac{1- \eps}{1+\eps}\right)^k &\approx& e^{\alpha x} \\
  f_k &\approx& \frac{1 - e^{\alpha x}}{1 - e^{\alpha}}
\end{eqnarray}
Otherwise ($h > 2/|\alpha|$), we get an oscillating solution, since $\gamma < 0$.
\subsection{Upwind difference}
We write:
\begin{eqnarray}
\frac{f_{k-1}-2f_k+f_{k+1}}{h^2} - \alpha \frac{f_k - f_{k-1}}{h} &=& 0 \\
(f_{k-1}-2f_k+f_{k+1}) - \alpha h (f_k - f_{k-1}) &=& 0 \\
(1 + 2\eps)f_{k-1}- (2 + 2\eps)f_k + f_{k+1} &=& 0 \\
2\eps = \alpha h
\end{eqnarray}
Again, write $f_k = \gamma^k$ to get:
\begin{eqnarray}
 \gamma^2 - (2 + 2\eps) \gamma + (1 + 2\eps) &=& 0
\end{eqnarray}
\begin{eqnarray}
\gamma &=& 1+\eps \pm \sqrt{(1+\eps)^2 - 1 - 2\eps} = 1 + \eps \pm |\eps| \in \{1, 1+2\eps\}
\end{eqnarray}
Given $\alpha > 0$, we note that there are no oscillations since $\gamma > 0$.

Moreover, the solution for $f_0 = 0$ and $f_N = 1$ (where $h N = 1$) is:
\begin{eqnarray}
f_k &=& \frac{1 - (1+2\eps)^k}{1 - (1+2\eps)^N}
\end{eqnarray}
Since $(1+2\eps)^k = (1+\alpha h)^k = \left(1 + \frac{\alpha}{N}\right)^k \approx e^{\alpha x}$ for $x = k/N$
so we get that $f_k \rightarrow f(x)$, as desired.
\subsection{Second order upwind scheme}
Suppose $f(x) = ax^2 + bx + c$:
\begin{eqnarray}
  f(0) &=& c \\
  f(-h) &=& ah^2 - bh + c \\
  f(-2h) &=& 4ah^2 - 2bh + c
\end{eqnarray}
Note that:
\begin{eqnarray}
  f(0) - f(-h) &=& bh - ah^2 \\
  f(0) - f(-2h) &=& 2bh - 4ah^2
\end{eqnarray}
This way we get 2nd order upwind approximation for the derivative $f'(0) = b$:
\begin{eqnarray}
  2bh &=& 4\left\{f(0) - f(-h)\right\} - \left\{f(0) - f(-2h)\right\} \\
  b &=& \frac{3f(0) - 4f(-h) + f(-2h)}{2h}
\end{eqnarray}
